Weidenbach_Book/IsaSAT_CDCL.thy
@@ -71,12 +71,6 @@ sepref_definition cdcl_twl_o_prog_wl_D_fast_code
 declare cdcl_twl_o_prog_wl_D_code.refine[sepref_fr_rules]
   cdcl_twl_o_prog_wl_D_fast_code.refine[sepref_fr_rules]
 
-lemma twl_st_heur_count_decided_st_alt_def:
-  fixes S :: twl_st_wl_heur
-  shows \<open>(S, T) \<in> twl_st_heur \<Longrightarrow> count_decided_st_heur S = count_decided (get_trail_wl T)\<close>
-  unfolding count_decided_st_def twl_st_heur_def trail_pol_def
-  by (cases S) (auto simp: count_decided_st_heur_def)
-
 lemma twl_st_heur''D_twl_st_heurD:
   assumes H: \<open>(\<And>\<D> r. f \<in> twl_st_heur'' \<D> r \<rightarrow>\<^sub>f \<langle>twl_st_heur'' \<D> r\<rangle> nres_rel)\<close>
   shows \<open>f \<in> twl_st_heur \<rightarrow>\<^sub>f \<langle>twl_st_heur\<rangle> nres_rel\<close>  (is \<open>_ \<in> ?A B\<close>)
